theories/logrel/fundamental.v
@@ -11,29 +11,48 @@ Section fundamental.
   Context `{hypparams:!HypervisorParameters}.
   Context `{vmG: !gen_VMG Σ}.
 
-  (* Global Instance VMProp_timeless id Q q: Timeless (VMProp id Q q). *)
-  (* Proof. rewrite /VMProp. admit.  Admitted. *)
-
   Lemma ftlr (i:VMID) (pgt:page_table) (regs: reg_file):
     interp_access i pgt regs⊢ interp_execute i.
   Proof.
     rewrite /interp_access /=.
-    iIntros "((%Hreg_full & regs) & VMProp) Hnotp VMProp_holds".
+    iIntros "((%Hreg_full & regs) & %Hpgt_full & VMProp) Hnotp VMProp_holds".
     iDestruct (VMProp_holds_agree i with "[VMProp_holds VMProp]") as "[Hres VMProp]".
     { iFrame. }
     iDestruct( later_or with "Hres") as "Hres".
     iDestruct "Hres" as "[Hres| >False]";last done.
-    { (* the vm is scheduled *)
-      rewrite !later_sep.
-      (* we have to do this because VMProp is not(?) timeless *)
-      iDestruct "Hres" as "(>R0z & >R1z & VMPropz)".
-      (* getting the PC *)
-      pose proof (Hlookup_PC:= (Hreg_full PC)).
-      simpl in Hlookup_PC.
-      destruct Hlookup_PC as [ai Hlookup_PC].
-      rewrite (big_opM_delete _ _ PC ai Hlookup_PC).
-      iDestruct ("regs") as "[PC regs]".
-
+    (* the vm is scheduled *)
+    rewrite !later_sep.
+    (* we have to do this because VMProp is not(?) timeless *)
+    iDestruct "Hres" as "(>R0z & >R1z & (VMPropz & >excl_pages & >shared_pages))".
+    (* getting the PC *)
+    pose proof (Hlookup_PC:= (Hreg_full PC)).
+    simpl in Hlookup_PC.
+    destruct Hlookup_PC as [ai Hlookup_PC].
+    rewrite (big_opM_delete _ _ PC ai Hlookup_PC).
+    iDestruct ("regs") as "[PC regs]".
+    (* getting sacc from pgt *)
+    pose proof (Hpgt_full (to_pid_aligned ai)) as Hlookup_ai.
+    simpl in Hlookup_ai.
+    destruct Hlookup_ai as [[? sacc] Hlookup_ai].
+    (* sswp *)
+    rewrite wp_sswp.
+    (* if i has access *)
+    destruct (decide (i ∈ sacc)).
+    { admit. }
+    {
+      iClear "VMProp VMPropz".
+      rewrite /shared_or_noaccess_pages.
+      rewrite (big_opM_delete _ _ (to_pid_aligned ai) _ Hlookup_ai).
+      iDestruct ("shared_pages") as "[pi shared_pages]".
+      simpl.
+      iDestruct ("pi" with "[]") as "[pi _]".
+      iPureIntro.
+      left;done.
+      iApply (not_valid_pc with "[PC pi]");
+      [exact n|iFrame|].
+      iNext;simpl.
+      iIntros "? _".
+      by iApply wp_terminated.
     }
 
 End fundamental.
